reduced the amount of abstraction in order to preserve sanity.

src/specs/seq.fst
@@ -17,60 +17,58 @@
 
 module Tesseract.Specs.Seq
 
-   type _spec_g (element_t: Type) =
-      Map.map_g nat element_t
+   type _spec_g (element_t: Type) 
+      = Map.map_g nat element_t
 
-   type _seq_g (element_t: Type) = 
-      { 
-         spec: _spec_g element_t;
-         length: nat
-      }
+   type _seq_g (element_t: Type) 
+      = 
+         { 
+            spec: _spec_g element_t;
+            length: nat
+         }
 
-   type is_seq_safe: #element_t: Type -> spec: _spec_g element_t -> length: nat -> Type =
-      fun (element_t: Type) (spec: _spec_g element_t) (length: nat) ->
-         forall (index: nat).
-            ((index < length) <==> (is_Some (spec index)))
-            /\ ((index >= length) <==> (None = (spec index)))
+   type is_seq_safe: #element_t: Type -> spec: _spec_g element_t -> length: nat -> Type 
+      =
+         fun (element_t: Type) (spec: _spec_g element_t) (length: nat) ->
+            forall (index: nat).
+               ((index < length) <==> (is_Some (spec index)))
+               /\ ((index >= length) <==> (None = (spec index)))
 
-   (*type is_seq_safe: #element_t: Type -> _seq_g element_t -> Type =
-      fun (element_t: Type) (seq: _seq_g element_t) ->
-         forall (index: nat).
-            ((index < seq.length) <==> (is_Some (seq.spec index)))
-            /\ ((index >= seq.length) <==> (None = (seq.spec index)))*)
-
-   type seq_g (element_t: Type) = 
-      seq: _seq_g element_t{is_seq_safe seq.spec seq.length}
+   type seq_g (element_t: Type) 
+      = seq: _seq_g element_t{is_seq_safe seq.spec seq.length}
 
    val bless:
       #element_t: Type ->
       spec: _spec_g element_t -> length: nat{is_seq_safe spec length} -> Tot (seq_g element_t)
-   let bless spec length =
-      {
-         spec = spec;
-         length = length
-      }
+   let bless spec length 
+      =
+         {
+            spec = spec;
+            length = length
+         }
 
    val empty: #element_t: Type -> Tot (seq_g element_t)
-   let empty (element_t: Type) = 
-      bless (fun _ -> None) 0
+   let empty (element_t: Type) 
+      = bless (fun _ -> None) 0
 
    val single: 
       #element_t: Type -> 
       element_t -> Tot (seq_g element_t)
-   let single lmnt =
-      bless
-         (fun index ->
-            if 0 = index then
-               Some lmnt
-            else
-               None)
-         1
+   let single lmnt 
+      =
+         bless
+            (fun index ->
+               if 0 = index then
+                  Some lmnt
+               else
+                  None)
+            1
 
    val length: 
       #element_t: Type -> 
       seq_g element_t -> Tot nat
-   let length (element_t: Type) seq = 
-      seq.length
+   let length (element_t: Type) seq 
+      = seq.length
 
    let to_map seq = seq.spec
    let lookup seq = seq.spec
@@ -79,84 +77,105 @@ module Tesseract.Specs.Seq
       #element_t: Type -> 
       seq: seq_g element_t -> index: nat{index < length seq} 
          -> Tot element_t
-   let nth (element_t: Type) seq index = 
-      match lookup seq index with
-         | Some lmnt ->
-            lmnt
+   let nth (element_t: Type) seq index
+      = 
+         match lookup seq index with
+            | Some lmnt ->
+               lmnt
 
    val first: 
       #element_t: Type -> 
          seq: seq_g element_t{0 < length seq} 
          -> Tot element_t
-   let first (element_t: Type) seq =
-      nth seq 0
+   let first (element_t: Type) seq 
+      = nth seq 0
 
    val last: 
       #element_t: Type -> 
          seq: seq_g element_t{0 < length seq} 
          -> Tot element_t
-   let last (element_t: Type) seq =
-      nth seq ((length seq) - 1)
+   let last (element_t: Type) seq 
+      = nth seq ((length seq) - 1)
 
    val append: 
       #element_t: Type -> 
          seq_g element_t -> element_t -> Tot (seq_g element_t)
-   let append (element_t: Type) seq lmnt =
-      bless
-         (fun index -> 
-            if index = seq.length then 
-               Some lmnt 
-            else 
-               lookup seq index)
-         (seq.length + 1)
+   let append (element_t: Type) seq lmnt 
+      =
+         bless
+            (fun index -> 
+               if index = seq.length then 
+                  Some lmnt 
+               else 
+                  lookup seq index)
+            (seq.length + 1)
 
    val concat: 
       #element_t: Type
       -> seq_g element_t -> seq_g element_t
       -> Tot (seq_g element_t)
-   let concat lhs rhs =
-      bless
-         (fun index ->
-            if index < lhs.length then
-               lhs.spec index
-            else
-               rhs.spec (index - lhs.length))
-         (lhs.length + rhs.length)
+   let concat lhs rhs 
+      =
+         bless
+            (fun index ->
+               if index < lhs.length then
+                  lhs.spec index
+               else
+                  rhs.spec (index - lhs.length))
+            (lhs.length + rhs.length)
 
    val _foldl__loop: 
       #element_t: Type -> #accum_t: Type -> 
       seq: seq_g element_t -> (accum_t -> element_t -> Tot accum_t) 
          -> accum_t -> index: nat{index < length seq}
          -> Tot accum_t (decreases index)
-   let rec _foldl__loop (element_t: Type) (accum_t: Type) seq fn accum index = 
-      if index = 0 then
-         accum
-      else
-         _foldl__loop seq fn (fn accum (nth seq index)) (index - 1)
+   let rec _foldl__loop (element_t: Type) (accum_t: Type) seq fn accum index 
+      = 
+         if index = 0 then
+            accum
+         else
+            _foldl__loop seq fn (fn accum (nth seq index)) (index - 1)
 
    val foldl: 
       #element_t: Type -> #accum_t: Type 
       -> (accum_t -> element_t -> Tot accum_t) -> accum_t -> seq_g element_t 
       -> Tot accum_t
-   let rec foldl (element_t: Type) (accum_t: Type) fn accum seq = 
-      let len = length seq in
-         if 0 = len then
-            accum
-         else
-            _foldl__loop seq fn accum (len - 1)
+   let rec foldl (element_t: Type) (accum_t: Type) fn accum seq 
+      = 
+         let len = length seq in
+            if 0 = len then
+               accum
+            else
+               _foldl__loop seq fn accum (len - 1)
 
    val filter: 
       #element_t: Type
-      -> seq_g element_t -> (element_t -> Tot bool)
+      -> (element_t -> Tot bool)
+      -> seq_g element_t 
       -> Tot (seq_g element_t)
-   let filter (element_t: Type) seq fn =
-      foldl
-         (fun (a: seq_g element_t) e ->
-            if fn e then
-               append a e
-            else
-               a)
-         Seq.empty
-         seq
+   let filter (element_t: Type) fn seq 
+      =
+         foldl
+            (fun (a: seq_g element_t) e ->
+               if fn e then
+                  append a e
+               else
+                  a)
+            Seq.empty
+            seq
+
+   val map:
+      #element0_t: Type
+      -> #element1_t: Type
+      -> (element0_t -> Tot element1_t)
+      -> seq_g element0_t
+      -> Tot (seq_g element1_t)
+   let map (element0_t: Type) (element1_t: Type) fn seq0
+      = 
+         foldl
+            (fun (accum: seq_g element1_t) element ->
+               Seq.append accum (fn element))
+            Seq.empty
+            seq0
 
 // $vim-fst:32: vim:set sts=3 sw=3 et ft=fstar:,$
