src/specs/history.fst
@@ -1,0 +1,125 @@
+// $legal:322:
+// 
+// This work is licensed under the Creative Commons
+// Attribution-NonCommercial-ShareAlike 4.0 International
+// License. To view a copy of this license, visit
+// http://creativecommons.org/licenses/by-nc-sa/4.0/
+// or send a letter to:
+// 
+// Creative Commons
+// PO Box 1866
+// Mountain View, CA 94042
+// USA
+// 
+// ,$
+
+//@requires "seq.fst"
+
+module Tesseract.Specs.History
+
+   type step_g (actor_id_t: Type) (message_t: Type) =
+      | Spawn: 
+         actor_id: actor_id_t 
+         -> step_g actor_id_t message_t
+      | Message: 
+         actor_id: actor_id_t 
+         -> message: message_t 
+         -> step_g actor_id_t message_t
+
+   type _history_g (actor_id_t: Type) (message_t: Type) =
+      {
+         steps: Seq.seq_g (step_g actor_id_t message_t);
+         known_ids: Set.set_g actor_id_t
+      }
+
+   type invariant: 
+      #actor_id_t: Type 
+      -> #message_t: Type 
+      -> _history_g actor_id_t message_t 
+      -> Type
+      = 
+         fun 
+            (actor_id_t: Type) 
+            (message_t: Type) 
+            (_history: 
+               _history_g actor_id_t message_t) 
+         ->
+            // each actor actor_id may only be spawned once.
+            (forall (actor_id: actor_id_t).
+               Set.is_mem _history.known_ids actor_id ==> 
+                  1 =
+                     Seq.foldl
+                        (fun accum event ->
+                           match event with
+                              | Spawn actor_id ->
+                                 accum + 1
+                              | _ ->
+                                 accum)
+                        0
+                        _history.steps)
+            // all actor ids must be in the set of known ids.
+            /\ (forall n.
+                  0 <= n && n < Seq.length _history.steps && is_Spawn (Seq.nth _history.steps n)
+                  ==>
+                     Set.is_mem _history.known_ids (Spawn.actor_id (Seq.nth _history.steps n)))
+
+   type history_g (actor_id_t: Type) (message_t: Type) 
+      = _history: _history_g actor_id_t message_t{invariant _history}
+
+   val init:
+      #actor_id_t: Type 
+      -> #message_t: Type 
+      -> Tot (history_g actor_id_t message_t)
+   let init 
+      (actor_id_t: Type) 
+      (message_t: Type) 
+      = 
+         {
+            steps = Seq.empty;
+            known_ids = Set.empty
+         }
+
+   val is_mem:
+      #actor_id_t: Type
+      -> #message_t: Type
+      -> history_g actor_id_t message_t
+      -> actor_id_t
+      -> Tot bool
+   let is_mem (actor_id_t: Type) (message_t: Type) history actor_id
+      = Set.is_mem history.known_ids actor_id
+
+   val local:
+      #actor_id_t: Type
+      -> #message_t: Type
+      -> history: history_g actor_id_t message_t
+      -> actor_id: actor_id_t{is_mem history actor_id}
+      -> Tot (Seq.seq_g (step_g actor_id_t message_t))
+   let local (actor_id_t: Type) (message_t: Type) history actor_id
+      = 
+         Seq.filter
+            (fun step ->
+               match step with
+                  | Spawn aid ->
+                     aid = actor_id
+                  | Message aid _ ->
+                     aid = actor_id)
+            history.steps
+
+   val global:
+      #actor_id_t: Type
+      -> #message_t: Type
+      -> history_g actor_id_t message_t
+      -> Tot (Seq.seq_g (step_g actor_id_t message_t))
+   let global (actor_id_t: Type) (message_t: Type) history
+      = history.steps
+
+// $vim-fst:32: vim:set sts=3 sw=3 et ft=fstar:,$
+
+
+
+
+
+
+
+
+
